Updating FlatAsm

x86/FlatAsm.v
@@ -8,239 +8,12 @@
 Require Import String Coqlib Maps.
 Require Import AST Integers Floats Values Memory Events Smallstep.
 Require Import Locations Stacklayout Conventions EraseArgs.
-Require Import Segment FlatAsmGlobenv FlatAsmBuiltin FlatAsmGlobdef.
+Require Import Segment FlatAsmGlobenv FlatAsmBuiltin.
 Require Import Asm RawAsm.
 Require Import Num.
 Require Globalenvs.
 
 
-(** * Abstract syntax *)
-
-(** A global location points to an offset in a segment *)
-Definition gloc:Type := seglabel.
-(** A label points to an offset in a segment. 
-    Labels are different from global locations in that they are local to a function *)
-Definition label:Type := seglabel.
-
-(** General form of an addressing mode. *)
-
-Inductive addrmode: Type :=
-  | Addrmode (base: option ireg)
-             (ofs: option (ireg * Z))
-             (const: Z + gloc * ptrofs).
-
-
-(** Instructions.  IA32 instructions accept many combinations of
-  registers, memory references and immediate constants as arguments.
-  Here, we list only the combinations that we actually use.
-
-  Naming conventions for types:
-- [b]: 8 bits
-- [w]: 16 bits ("word")
-- [l]: 32 bits ("longword")
-- [q]: 64 bits ("quadword")
-- [d] or [sd]: FP double precision (64 bits)
-- [s] or [ss]: FP single precision (32 bits)
-
-  Naming conventions for operands:
-- [r]: integer register operand
-- [f]: XMM register operand
-- [m]: memory operand
-- [i]: immediate integer operand
-- [s]: immediate symbol operand
-- [l]: immediate label operand
-- [cl]: the [CL] register
-
-  For two-operand instructions, the first suffix describes the result
-  (and first argument), the second suffix describes the second argument.
-*)
-
-Inductive instruction: Type :=
-  (** Moves *)
-  | Pmov_rr (rd: ireg) (r1: ireg)       (**r [mov] (integer) *)
-  | Pmovl_ri (rd: ireg) (n: int)
-  | Pmovq_ri (rd: ireg) (n: int64)
-  | Pmov_rs (rd: ireg) (loc: gloc)
-  | Pmovl_rm (rd: ireg) (a: addrmode)
-  | Pmovq_rm (rd: ireg) (a: addrmode)
-  | Pmovl_mr (a: addrmode) (rs: ireg)
-  | Pmovq_mr (a: addrmode) (rs: ireg)
-  | Pmovsd_ff (rd: freg) (r1: freg)     (**r [movsd] (single 64-bit float) *)
-  | Pmovsd_fi (rd: freg) (n: float)     (**r (pseudo-instruction) *)
-  | Pmovsd_fm (rd: freg) (a: addrmode)
-  | Pmovsd_mf (a: addrmode) (r1: freg)
-  | Pmovss_fi (rd: freg) (n: float32)   (**r [movss] (single 32-bit float) *)
-  | Pmovss_fm (rd: freg) (a: addrmode)
-  | Pmovss_mf (a: addrmode) (r1: freg)
-  | Pfldl_m (a: addrmode)               (**r [fld] double precision *)
-  | Pfstpl_m (a: addrmode)              (**r [fstp] double precision *)
-  | Pflds_m (a: addrmode)               (**r [fld] simple precision *)
-  | Pfstps_m (a: addrmode)              (**r [fstp] simple precision *)
-  | Pxchg_rr (r1: ireg) (r2: ireg)      (**r register-register exchange *)
-  (** Moves with conversion *)
-  | Pmovb_mr (a: addrmode) (rs: ireg)   (**r [mov] (8-bit int) *)
-  | Pmovw_mr (a: addrmode) (rs: ireg)   (**r [mov] (16-bit int) *)
-  | Pmovzb_rr (rd: ireg) (rs: ireg)     (**r [movzb] (8-bit zero-extension) *)
-  | Pmovzb_rm (rd: ireg) (a: addrmode)
-  | Pmovsb_rr (rd: ireg) (rs: ireg)     (**r [movsb] (8-bit sign-extension) *)
-  | Pmovsb_rm (rd: ireg) (a: addrmode)
-  | Pmovzw_rr (rd: ireg) (rs: ireg)     (**r [movzw] (16-bit zero-extension) *)
-  | Pmovzw_rm (rd: ireg) (a: addrmode)
-  | Pmovsw_rr (rd: ireg) (rs: ireg)     (**r [movsw] (16-bit sign-extension) *)
-  | Pmovsw_rm (rd: ireg) (a: addrmode)
-  | Pmovzl_rr (rd: ireg) (rs: ireg)     (**r [movzl] (32-bit zero-extension) *)
-  | Pmovsl_rr (rd: ireg) (rs: ireg)     (**r [movsl] (32-bit sign-extension) *)
-  | Pmovls_rr (rd: ireg)                (** 64 to 32 bit conversion (pseudo) *)
-  | Pcvtsd2ss_ff (rd: freg) (r1: freg)  (**r conversion to single float *)
-  | Pcvtss2sd_ff (rd: freg) (r1: freg)  (**r conversion to double float *)
-  | Pcvttsd2si_rf (rd: ireg) (r1: freg) (**r double to signed int *)
-  | Pcvtsi2sd_fr (rd: freg) (r1: ireg)  (**r signed int to double *)
-  | Pcvttss2si_rf (rd: ireg) (r1: freg) (**r single to signed int *)
-  | Pcvtsi2ss_fr (rd: freg) (r1: ireg)  (**r signed int to single *)
-  | Pcvttsd2sl_rf (rd: ireg) (r1: freg) (**r double to signed long *)
-  | Pcvtsl2sd_fr (rd: freg) (r1: ireg)  (**r signed long to double *)
-  | Pcvttss2sl_rf (rd: ireg) (r1: freg) (**r single to signed long *)
-  | Pcvtsl2ss_fr (rd: freg) (r1: ireg)  (**r signed long to single *)
-  (** Integer arithmetic *)
-  | Pleal (rd: ireg) (a: addrmode)
-  | Pleaq (rd: ireg) (a: addrmode)
-  | Pnegl (rd: ireg)
-  | Pnegq (rd: ireg)
-  | Paddl_ri (rd: ireg) (n: int)
-  | Paddq_ri (rd: ireg) (n: int64)
-  | Psubl_rr (rd: ireg) (r1: ireg)
-  | Psubq_rr (rd: ireg) (r1: ireg)
-  | Pimull_rr (rd: ireg) (r1: ireg)
-  | Pimulq_rr (rd: ireg) (r1: ireg)
-  | Pimull_ri (rd: ireg) (n: int)
-  | Pimulq_ri (rd: ireg) (n: int64)
-  | Pimull_r (r1: ireg)
-  | Pimulq_r (r1: ireg)
-  | Pmull_r (r1: ireg)
-  | Pmulq_r (r1: ireg)
-  | Pcltd
-  | Pcqto
-  | Pdivl (r1: ireg)
-  | Pdivq (r1: ireg)
-  | Pidivl (r1: ireg)
-  | Pidivq (r1: ireg)
-  | Pandl_rr (rd: ireg) (r1: ireg)
-  | Pandq_rr (rd: ireg) (r1: ireg)
-  | Pandl_ri (rd: ireg) (n: int)
-  | Pandq_ri (rd: ireg) (n: int64)
-  | Porl_rr (rd: ireg) (r1: ireg)
-  | Porq_rr (rd: ireg) (r1: ireg)
-  | Porl_ri (rd: ireg) (n: int)
-  | Porq_ri (rd: ireg) (n: int64)
-  | Pxorl_r (rd: ireg)                  (**r [xor] with self = set to zero *)
-  | Pxorq_r (rd: ireg)
-  | Pxorl_rr (rd: ireg) (r1: ireg)
-  | Pxorq_rr (rd: ireg) (r1: ireg)
-  | Pxorl_ri (rd: ireg) (n: int)
-  | Pxorq_ri (rd: ireg) (n: int64)
-  | Pnotl (rd: ireg)
-  | Pnotq (rd: ireg)
-  | Psall_rcl (rd: ireg)
-  | Psalq_rcl (rd: ireg)
-  | Psall_ri (rd: ireg) (n: int)
-  | Psalq_ri (rd: ireg) (n: int)
-  | Pshrl_rcl (rd: ireg)
-  | Pshrq_rcl (rd: ireg)
-  | Pshrl_ri (rd: ireg) (n: int)
-  | Pshrq_ri (rd: ireg) (n: int)
-  | Psarl_rcl (rd: ireg)
-  | Psarq_rcl (rd: ireg)
-  | Psarl_ri (rd: ireg) (n: int)
-  | Psarq_ri (rd: ireg) (n: int)
-  | Pshld_ri (rd: ireg) (r1: ireg) (n: int)
-  | Prorl_ri (rd: ireg) (n: int)
-  | Prorq_ri (rd: ireg) (n: int)
-  | Pcmpl_rr (r1 r2: ireg)
-  | Pcmpq_rr (r1 r2: ireg)
-  | Pcmpl_ri (r1: ireg) (n: int)
-  | Pcmpq_ri (r1: ireg) (n: int64)
-  | Ptestl_rr (r1 r2: ireg)
-  | Ptestq_rr (r1 r2: ireg) 
-  | Ptestl_ri (r1: ireg) (n: int)
-  | Ptestq_ri (r1: ireg) (n: int64)
-  | Pcmov (c: testcond) (rd: ireg) (r1: ireg)
-  | Psetcc (c: testcond) (rd: ireg)
-  (** Floating-point arithmetic *)
-  | Paddd_ff (rd: freg) (r1: freg)
-  | Psubd_ff (rd: freg) (r1: freg)
-  | Pmuld_ff (rd: freg) (r1: freg)
-  | Pdivd_ff (rd: freg) (r1: freg)
-  | Pnegd (rd: freg)
-  | Pabsd (rd: freg)
-  | Pcomisd_ff (r1 r2: freg)
-  | Pxorpd_f (rd: freg)	              (**r [xor] with self = set to zero *)
-  | Padds_ff (rd: freg) (r1: freg)
-  | Psubs_ff (rd: freg) (r1: freg)
-  | Pmuls_ff (rd: freg) (r1: freg)
-  | Pdivs_ff (rd: freg) (r1: freg)
-  | Pnegs (rd: freg)
-  | Pabss (rd: freg)
-  | Pcomiss_ff (r1 r2: freg)
-  | Pxorps_f (rd: freg)	              (**r [xor] with self = set to zero *)
-  (** Branches and calls *)
-  | Pjmp_l (l: label)
-  | Pjmp_s (loc: gloc) (sg: signature)
-  | Pjmp_r (r: ireg) (sg: signature)
-  | Pjcc (c: testcond)(l: label)
-  | Pjcc2 (c1 c2: testcond)(l: label)   (**r pseudo *)
-  | Pjmptbl (r: ireg) (tbl: list label) (**r pseudo *)
-  | Pcall_s (loc: gloc) (sg: signature)
-  | Pcall_r (r: ireg) (sg: signature)
-  | Pret
-  (** Saving and restoring registers *)
-  | Pmov_rm_a (rd: ireg) (a: addrmode)  (**r like [Pmov_rm], using [Many64] chunk *)
-  | Pmov_mr_a (a: addrmode) (rs: ireg)  (**r like [Pmov_mr], using [Many64] chunk *)
-  | Pmovsd_fm_a (rd: freg) (a: addrmode) (**r like [Pmovsd_fm], using [Many64] chunk *)
-  | Pmovsd_mf_a (a: addrmode) (r1: freg) (**r like [Pmovsd_mf], using [Many64] chunk *)
-  (** Pseudo-instructions *)
-  | Plabel(l: label)
-  | Pallocframe(frame: frame_info)(ofs_ra: ptrofs)
-  | Pfreeframe (sz: Z) (ofs_ra: ptrofs)
-  | Pload_parent_pointer (rd: ireg) (sz:Z)
-  | Pbuiltin(ef: external_function)(args: list (builtin_arg preg))(res: builtin_res preg)
-  (** Instructions not generated by [Asmgen] -- TO CHECK *)
-  | Padcl_ri (rd: ireg) (n: int)
-  | Padcl_rr (rd: ireg) (r2: ireg)
-  | Paddl_mi (a: addrmode) (n: int)
-  | Paddl_rr (rd: ireg) (r2: ireg)
-  | Pbsfl (rd: ireg) (r1: ireg)
-  | Pbsfq (rd: ireg) (r1: ireg)
-  | Pbsrl (rd: ireg) (r1: ireg)
-  | Pbsrq (rd: ireg) (r1: ireg)
-  | Pbswap64 (rd: ireg)
-  | Pbswap32 (rd: ireg)
-  | Pbswap16 (rd: ireg)
-  | Pcfi_adjust (n: int)
-  | Pfmadd132 (rd: freg) (r2: freg) (r3: freg)
-  | Pfmadd213 (rd: freg) (r2: freg) (r3: freg)
-  | Pfmadd231 (rd: freg) (r2: freg) (r3: freg)
-  | Pfmsub132 (rd: freg) (r2: freg) (r3: freg)
-  | Pfmsub213 (rd: freg) (r2: freg) (r3: freg)
-  | Pfmsub231 (rd: freg) (r2: freg) (r3: freg)
-  | Pfnmadd132 (rd: freg) (r2: freg) (r3: freg)
-  | Pfnmadd213 (rd: freg) (r2: freg) (r3: freg)
-  | Pfnmadd231 (rd: freg) (r2: freg) (r3: freg)
-  | Pfnmsub132 (rd: freg) (r2: freg) (r3: freg)
-  | Pfnmsub213 (rd: freg) (r2: freg) (r3: freg)
-  | Pfnmsub231 (rd: freg) (r2: freg) (r3: freg)
-  | Pmaxsd (rd: freg) (r2: freg)
-  | Pminsd (rd: freg) (r2: freg)
-  | Pmovb_rm (rd: ireg) (a: addrmode)
-  | Pmovsq_mr  (a: addrmode) (rs: freg)
-  | Pmovsq_rm (rd: freg) (a: addrmode)
-  | Pmovsb
-  | Pmovsw
-  | Pmovw_rm (rd: ireg) (ad: addrmode)
-  | Prep_movsl
-  | Psbbl_rr (rd: ireg) (r2: ireg)
-  | Psqrtsd (rd: freg) (r1: freg)
-  | Psubl_ri (rd: ireg) (n: int)
-  | Psubq_ri (rd: ireg) (n: int64).
 
 Definition instr_with_info:Type := instruction * segblock.
 Definition code := list instr_with_info.
@@ -248,16 +21,20 @@ Record function : Type := mkfunction { fn_sig: signature; fn_code: code; fn_fram
 Definition fundef := AST.fundef function.
 Definition gdef := (FlatAsmGlobdef.globdef fundef unit).
 
+(* mapping from global identifiers to segment labels *)
+Definition GID_MAP_TYPE := ident -> option seglabel.
+(* mapping from local labels to segment labels *)
+Definition LABEL_MAP_TYPE := ident -> ident -> option seglabel.
 
 (* The FlatAsm program *)
 Record program : Type := {
-  prog_defs: list (ident * option gdef * segblock);
+  prog_defs: list (ident * option gdef);
   prog_public: list ident;
   prog_main: ident;
-  (* stack_seg: segment; (* The stack segment *) *)
   data_seg: segment;  (* The data segment *)
-  code_seg : segment * code; (* The code segment *)
-  extfuns_seg : segment; (* The segment for external functions *)
+  code_seg: segment * code; (* The code segment *)
+  glob_map: GID_MAP_TYPE;
+  lbl_map: LABEL_MAP_TYPE;
   prog_senv : Globalenvs.Senv.t;
 }.
 
@@ -265,7 +42,7 @@ Record program : Type := {
 (** * Operational semantics *)
 
 (* Definition regset := Asm.regset. *)
-Definition genv := Genv.t fundef instr_with_info.
+Definition genv := Genv.t fundef unit instr_with_info.
 
 Notation "a # b" := (a b) (at level 1, only parsing) : asm.
 Notation "a # b <- c" := (Asm.Pregmap.set b c a) (at level 1, b at next level) : asm.
@@ -281,8 +58,8 @@ Section RELSEM.
 
 Section WITHGE.
 
-Context {F I: Type}.
-Variable ge: Genv.t F I.
+Context {F V I: Type}.
+Variable ge: Genv.t F V I.
   
 (** Evaluating an addressing mode *)
 
@@ -301,7 +78,7 @@ Definition eval_addrmode32 (a: addrmode) (rs: regset) : val :=
              end)
            (match const with
             | inl ofs => Vint (Int.repr ofs)
-            | inr(gloc, ofs) => Genv.symbol_address ge gloc ofs
+            | inr(id, ofs) => Genv.symbol_address ge id ofs
             end)).
 
 Definition eval_addrmode64 (a: addrmode) (rs: regset) : val :=
@@ -319,7 +96,7 @@ Definition eval_addrmode64 (a: addrmode) (rs: regset) : val :=
              end)
            (match const with
             | inl ofs => Vlong (Int64.repr ofs)
-            | inr(gloc, ofs) => Genv.symbol_address ge gloc ofs
+            | inr(id, ofs) => Genv.symbol_address ge id ofs
             end)).
 
 Definition eval_addrmode (a: addrmode) (rs: regset) : val :=
@@ -339,8 +116,16 @@ End WITHGE.
   [nextinstr_nf] is a variant of [nextinstr] that sets condition flags
   to [Vundef] in addition to incrementing the [PC]. *)
 
-Definition goto_label {F I} (ge: Genv.t F I) (lbl: label) (rs: regset) (m: mem) :=
-  Next (rs#PC <- (Genv.symbol_address ge lbl Ptrofs.zero)) m.
+Definition goto_label {F V I} (ge: Genv.t F V I) (fid: ident) (lbl: label) (rs: regset) (m: mem) :=
+  match Genv.genv_lbl ge fid lbl with
+  | None => Stuck
+  | Some (b, ofs) =>
+      match rs#PC with
+      | Vptr b ofs => Next (rs#PC <- (Vptr b ofs)) m
+      | _ => Stuck
+    end
+  end.
+
 
 (** [CompCertiKOS:test-compcert-param-mem-accessors] For CertiKOS, we
 need to parameterize over [exec_load] and [exec_store], which will be
@@ -349,8 +134,8 @@ mode. *)
 
 Class MemAccessors
       `{!Mem.MemoryModelOps mem}
-      (exec_load: forall F I: Type, Genv.t F I -> memory_chunk -> mem -> addrmode -> regset -> preg -> ptrofs -> outcome)
-      (exec_store: forall F I: Type, Genv.t F I -> memory_chunk -> mem -> addrmode -> regset -> preg -> list preg -> ptrofs -> outcome)
+      (exec_load: forall F V I: Type, Genv.t F V I -> memory_chunk -> mem -> addrmode -> regset -> preg -> ptrofs -> outcome)
+      (exec_store: forall F V I: Type, Genv.t F V I -> memory_chunk -> mem -> addrmode -> regset -> preg -> list preg -> ptrofs -> outcome)
 : Prop := {}.
 
 Section MEM_ACCESSORS_DEFAULT.
@@ -359,14 +144,14 @@ Section MEM_ACCESSORS_DEFAULT.
 care about kernel vs. user mode, and uses its memory model to define
 its memory accessors. *)
 
-Definition exec_load {F I} (ge: Genv.t F I) (chunk: memory_chunk) (m: mem)
+Definition exec_load {F V I} (ge: Genv.t F V I) (chunk: memory_chunk) (m: mem)
                      (a: addrmode) (rs: regset) (rd: preg) (sz:ptrofs):=
   match Mem.loadv chunk m (eval_addrmode ge a rs) with
   | Some v => Next (nextinstr_nf (rs#rd <- v) sz) m
   | None => Stuck
   end.
 
-Definition exec_store {F I} (ge: Genv.t F I) (chunk: memory_chunk) (m: mem)
+Definition exec_store {F V I} (ge: Genv.t F V I) (chunk: memory_chunk) (m: mem)
                       (a: addrmode) (rs: regset) (r1: preg)
                       (destroyed: list preg) (sz:ptrofs) :=
   match Mem.storev chunk m (eval_addrmode ge a rs) (rs r1) with
@@ -399,7 +184,7 @@ End MEM_ACCESSORS_DEFAULT.
     but we do not need to model this precisely.
 *)
 
-Definition exec_instr {exec_load exec_store} `{!MemAccessors exec_load exec_store} (ge: genv) (ii: instr_with_info) (rs: regset) (m: mem) : outcome :=
+Definition exec_instr {exec_load exec_store} `{!MemAccessors exec_load exec_store} (ge: genv) (fid:ident) (ii: instr_with_info) (rs: regset) (m: mem) : outcome :=
   let (i,blk) := ii in
   let sz := segblock_size blk in
   match i with
@@ -410,61 +195,61 @@ Definition exec_instr {exec_load exec_store} `{!MemAccessors exec_load exec_stor
       Next (nextinstr_nf (rs#rd <- (Vint n)) sz) m
   | Pmovq_ri rd n =>
       Next (nextinstr_nf (rs#rd <- (Vlong n)) sz) m
-  | Pmov_rs rd gloc =>
-      Next (nextinstr_nf (rs#rd <- (Genv.symbol_address ge gloc Ptrofs.zero)) sz) m
+  | Pmov_rs rd id =>
+      Next (nextinstr_nf (rs#rd <- (Genv.symbol_address ge id Ptrofs.zero)) sz) m
   | Pmovl_rm rd a =>
-      exec_load _ _ ge Mint32 m a rs rd sz
+      exec_load _ _ _ ge Mint32 m a rs rd sz
   | Pmovq_rm rd a =>
-      exec_load _ _ ge Mint64 m a rs rd sz
+      exec_load _ _ _ ge Mint64 m a rs rd sz
   | Pmovl_mr a r1 =>
-      exec_store _ _ ge Mint32 m a rs r1 nil sz
+      exec_store _ _ _ ge Mint32 m a rs r1 nil sz
   | Pmovq_mr a r1 =>
-      exec_store _ _ ge Mint64 m a rs r1 nil sz
+      exec_store _ _ _ ge Mint64 m a rs r1 nil sz
   | Pmovsd_ff rd r1 =>
       Next (nextinstr (rs#rd <- (rs r1)) sz) m
   | Pmovsd_fi rd n =>
       Next (nextinstr (rs#rd <- (Vfloat n)) sz) m
   | Pmovsd_fm rd a =>
-      exec_load _ _ ge Mfloat64 m a rs rd  sz
+      exec_load _ _ _ ge Mfloat64 m a rs rd  sz
   | Pmovsd_mf a r1 =>
-      exec_store _ _ ge Mfloat64 m a rs r1 nil sz
+      exec_store _ _ _ ge Mfloat64 m a rs r1 nil sz
   | Pmovss_fi rd n =>
       Next (nextinstr (rs#rd <- (Vsingle n)) sz) m
   | Pmovss_fm rd a =>
-      exec_load _ _ ge Mfloat32 m a rs rd sz
+      exec_load _ _ _ ge Mfloat32 m a rs rd sz
   | Pmovss_mf a r1 =>
-      exec_store _ _ ge Mfloat32 m a rs r1 nil sz
+      exec_store _ _ _ ge Mfloat32 m a rs r1 nil sz
   | Pfldl_m a =>
-      exec_load _ _ ge Mfloat64 m a rs ST0 sz
+      exec_load _ _ _ ge Mfloat64 m a rs ST0 sz
   | Pfstpl_m a =>
-      exec_store _ _ ge Mfloat64 m a rs ST0 (ST0 :: nil) sz
+      exec_store _ _ _ ge Mfloat64 m a rs ST0 (ST0 :: nil) sz
   | Pflds_m a =>
-      exec_load _ _ ge Mfloat32 m a rs ST0 sz
+      exec_load _ _ _ ge Mfloat32 m a rs ST0 sz
   | Pfstps_m a =>
-      exec_store _ _ ge Mfloat32 m a rs ST0 (ST0 :: nil) sz
+      exec_store _ _ _ ge Mfloat32 m a rs ST0 (ST0 :: nil) sz
   | Pxchg_rr r1 r2 =>
       Next (nextinstr (rs#r1 <- (rs r2) #r2 <- (rs r1)) sz) m
   (** Moves with conversion *)
   | Pmovb_mr a r1 =>
-      exec_store _ _ ge Mint8unsigned m a rs r1 nil sz
+      exec_store _ _ _ ge Mint8unsigned m a rs r1 nil sz
   | Pmovw_mr a r1 =>
-      exec_store _ _ ge Mint16unsigned m a rs r1 nil sz
+      exec_store _ _ _ ge Mint16unsigned m a rs r1 nil sz
   | Pmovzb_rr rd r1 =>
       Next (nextinstr (rs#rd <- (Val.zero_ext 8 rs#r1)) sz) m
   | Pmovzb_rm rd a =>
-      exec_load _ _ ge Mint8unsigned m a rs rd sz
+      exec_load _ _ _ ge Mint8unsigned m a rs rd sz
   | Pmovsb_rr rd r1 =>
       Next (nextinstr (rs#rd <- (Val.sign_ext 8 rs#r1)) sz) m
   | Pmovsb_rm rd a =>
-      exec_load _ _ ge Mint8signed m a rs rd sz
+      exec_load _ _ _ ge Mint8signed m a rs rd sz
   | Pmovzw_rr rd r1 =>
       Next (nextinstr (rs#rd <- (Val.zero_ext 16 rs#r1)) sz) m
   | Pmovzw_rm rd a =>
-      exec_load _ _ ge Mint16unsigned m a rs rd sz
+      exec_load _ _ _ ge Mint16unsigned m a rs rd sz
   | Pmovsw_rr rd r1 =>
       Next (nextinstr (rs#rd <- (Val.sign_ext 16 rs#r1)) sz) m
   | Pmovsw_rm rd a =>
-      exec_load _ _ ge Mint16signed m a rs rd sz
+      exec_load _ _ _ ge Mint16signed m a rs rd sz
   | Pmovzl_rr rd r1 =>
       Next (nextinstr (rs#rd <- (Val.longofintu rs#r1)) sz) m
   | Pmovsl_rr rd r1 =>
@@ -696,20 +481,20 @@ Definition exec_instr {exec_load exec_store} `{!MemAccessors exec_load exec_stor
       Next (nextinstr_nf (rs#rd <- (Vsingle Float32.zero)) sz) m
   (** Branches and calls *)
   | Pjmp_l lbl =>
-      goto_label ge lbl rs m
-  | Pjmp_s gloc sg =>
-      Next (rs#PC <- (Genv.symbol_address ge gloc Ptrofs.zero)) m
+      goto_label ge fid lbl rs m
+  | Pjmp_s id sg =>
+      Next (rs#PC <- (Genv.symbol_address ge id Ptrofs.zero)) m
   | Pjmp_r r sg =>
       Next (rs#PC <- (rs r)) m
   | Pjcc cond lbl =>
       match eval_testcond cond rs with
-      | Some true => goto_label ge lbl rs m
+      | Some true => goto_label ge fid lbl rs m
       | Some false => Next (nextinstr rs sz) m
       | None => Stuck
       end
   | Pjcc2 cond1 cond2 lbl =>
       match eval_testcond cond1 rs, eval_testcond cond2 rs with
-      | Some true, Some true => goto_label ge lbl rs m
+      | Some true, Some true => goto_label ge fid lbl rs m
       | Some _, Some _ => Next (nextinstr rs sz) m
       | _, _ => Stuck
       end
@@ -718,7 +503,7 @@ Definition exec_instr {exec_load exec_store} `{!MemAccessors exec_load exec_stor
       | Vint n =>
           match list_nth_z tbl (Int.unsigned n) with
           | None => Stuck
-          | Some lbl => goto_label ge lbl (rs #RAX <- Vundef #RDX <- Vundef) m
+          | Some lbl => goto_label ge fid lbl (rs #RAX <- Vundef #RDX <- Vundef) m
           end
       | _ => Stuck
       end
@@ -732,13 +517,13 @@ Definition exec_instr {exec_load exec_store} `{!MemAccessors exec_load exec_stor
       Next (rs#PC <- (rs#RA) #RA <- Vundef) m
   (** Saving and restoring registers *)
   | Pmov_rm_a rd a =>
-      exec_load _ _ ge (if Archi.ptr64 then Many64 else Many32) m a rs rd sz
+      exec_load _ _ _ ge (if Archi.ptr64 then Many64 else Many32) m a rs rd sz
   | Pmov_mr_a a r1 =>
-      exec_store _ _ ge (if Archi.ptr64 then Many64 else Many32) m a rs r1 nil sz
+      exec_store _ _ _ ge (if Archi.ptr64 then Many64 else Many32) m a rs r1 nil sz
   | Pmovsd_fm_a rd a =>
-      exec_load _ _ ge Many64 m a rs rd sz
+      exec_load _ _ _  ge Many64 m a rs rd sz
   | Pmovsd_mf_a a r1 =>
-      exec_store _ _ ge Many64 m a rs r1 nil sz
+      exec_store _ _ _ ge Many64 m a rs r1 nil sz
   (** Pseudo-instructions *)
   | Plabel lbl =>
       Next (nextinstr rs sz) m
@@ -807,18 +592,16 @@ Definition exec_instr {exec_load exec_store} `{!MemAccessors exec_load exec_stor
 Inductive step {exec_load exec_store} `{!MemAccessors exec_load exec_store} 
   (ge: genv) : state -> trace -> state -> Prop :=
 | exec_step_internal:
-    forall b ofs i rs m rs' m',
+    forall b fid ofs i rs m rs' m',
       rs PC = Vptr b ofs ->
-      Genv.genv_internal_codeblock ge b = true ->
-      Genv.find_instr ge (Vptr b ofs) = Some i ->
-      exec_instr ge i rs m = Next rs' m' ->
+      Genv.find_instr ge (Vptr b ofs) = Some (i,fid) ->
+      exec_instr ge fid i rs m = Next rs' m' ->
       step ge (State rs m) E0 (State rs' m')
 | exec_step_builtin:
-    forall b ofs ef args res rs m vargs t vres rs' m' blk,
+    forall fid b ofs ef args res rs m vargs t vres rs' m' blk,
       rs PC = Vptr b ofs ->
-      Genv.genv_internal_codeblock ge b = true ->
-      Genv.find_instr ge (Vptr b ofs) = Some (Pbuiltin ef args res, blk) ->
-      eval_builtin_args _ _ preg ge rs (rs RSP) m args vargs ->
+      Genv.find_instr ge (Vptr b ofs) = Some ((Pbuiltin ef args res, blk), fid)  ->
+      eval_builtin_args _ _ _ preg ge rs (rs RSP) m args vargs ->
         external_call ef (Genv.genv_senv ge) vargs m t vres m' ->
       forall BUILTIN_ENABLED: builtin_enabled ef,
         rs' = nextinstr_nf
@@ -828,7 +611,6 @@ Inductive step {exec_load exec_store} `{!MemAccessors exec_load exec_store}
 | exec_step_external:
     forall b ofs ef args res rs m t rs' m',
       rs PC = Vptr b ofs ->
-      Genv.genv_internal_codeblock ge b = false ->
       Genv.find_funct ge (Vptr b ofs) = Some (External ef) ->
       extcall_arguments rs m (ef_sig ef) args ->
       forall (* CompCertX: BEGIN additional conditions for calling convention *)
@@ -850,38 +632,37 @@ Inductive step {exec_load exec_store} `{!MemAccessors exec_load exec_store}
 End RELSEM.
 
 (** Initialization of the global environment *)
-Definition add_global (ge:genv) (idg: ident * option gdef * segblock) : genv :=
-  let '(gid,gdef,sb) := idg in
-  let ptr := Genv.symbol_address ge (segblock_to_label sb) Ptrofs.zero in
-  match gdef with
+Definition add_global (ge:genv) (idg: ident * option gdef) : genv :=
+  let '(gid,gdef) := idg in
+  match (Genv.genv_symb ge gid) with
   | None => ge
-  | Some (Gvar _) => ge
-  | Some (Gfun f) =>
+  | Some (b, ofs) =>
     (Genv.mkgenv
        (Genv.genv_public ge)
-       (fun b ofs => if Val.eq (Vptr b ofs) ptr then Some f else (Genv.genv_defs ge b ofs))
+       (Genv.genv_symb ge)
+       (fun b' ofs' => if (peq b b') && (Ptrofs.eq ofs ofs') then gdef else (Genv.genv_defs ge b ofs))
        (Genv.genv_instrs ge)
-       (Genv.genv_internal_codeblock ge)
-       (Genv.genv_segblocks ge)
+       (Genv.genv_lbl ge)
        (Genv.genv_next ge)
        (Genv.genv_senv ge))
   end.
-
-Fixpoint add_globals (ge:genv) (gl: list (ident * option gdef * segblock)) : genv :=
+    
+Fixpoint add_globals (ge:genv) (gl: list (ident * option gdef)) : genv :=
   match gl with
   | nil => ge
   | (idg::gl') => 
     let ge' := add_global ge idg in
     add_globals ge' gl'
-  end.  
+  end. 
 
 Lemma add_global_pres_genv_instrs: forall def ge ge',
   ge' = add_global ge def ->
   forall b ofs, Genv.genv_instrs ge b ofs = Genv.genv_instrs ge' b ofs.
 Proof.
   intros def ge ge' H b ofs.
-  subst. unfold add_global. destruct def. destruct p. destruct o.
-  destruct g. simpl. auto. auto. auto.
+  subst. unfold add_global. destruct def. 
+  destruct (Genv.genv_symb ge i) eqn:EQ.
+  destruct p. auto. auto.
 Qed.
 
 Lemma add_globals_pres_genv_instrs: forall defs ge ge',
@@ -895,25 +676,25 @@ Proof.
     rewrite H0. apply IHdefs. auto.
 Qed.
 
-Lemma add_global_pres_genv_segblocks: forall def ge ge',
-  ge' = add_global ge def ->
-  forall id, Genv.genv_segblocks ge id = Genv.genv_segblocks ge' id.
-Proof.
-  intros def ge ge' H id.
-  subst. unfold add_global. destruct def. destruct p. destruct o.
-  destruct g. simpl. auto. auto. auto.
-Qed.
+(* Lemma add_global_pres_genv_segblocks: forall def ge ge', *)
+(*   ge' = add_global ge def -> *)
+(*   forall id, Genv.genv_segblocks ge id = Genv.genv_segblocks ge' id. *)
+(* Proof. *)
+(*   intros def ge ge' H id. *)
+(*   subst. unfold add_global. destruct def. destruct p. destruct o. *)
+(*   destruct g. simpl. auto. auto. auto. *)
+(* Qed. *)
 
-Lemma add_globals_pres_genv_segblocks: forall defs ge ge',
-  ge' = add_globals ge defs ->
-  forall id, Genv.genv_segblocks ge id = Genv.genv_segblocks ge' id.
-Proof.
-  induction defs; simpl; intros.
-  - subst. auto.
-  - assert (Genv.genv_segblocks ge id = Genv.genv_segblocks (add_global ge a) id)
-           by (eapply add_global_pres_genv_segblocks; eauto).
-    rewrite H0. apply IHdefs. auto.
-Qed.
+(* Lemma add_globals_pres_genv_segblocks: forall defs ge ge', *)
+(*   ge' = add_globals ge defs -> *)
+(*   forall id, Genv.genv_segblocks ge id = Genv.genv_segblocks ge' id. *)
+(* Proof. *)
+(*   induction defs; simpl; intros. *)
+(*   - subst. auto. *)
+(*   - assert (Genv.genv_segblocks ge id = Genv.genv_segblocks (add_global ge a) id) *)
+(*            by (eapply add_global_pres_genv_segblocks; eauto). *)
+(*     rewrite H0. apply IHdefs. auto. *)
+(* Qed. *)
 
 Definition get_instr_ptr (smap:segid_type ->block) (i:instr_with_info): val :=
   let (_,bi) := i in Genv.label_to_ptr smap (segblock_to_label bi).
